Try new strategy for pattern substitution
Do individually instead of all at once
should be easier to reason about
Might have to pair pattern and term sub together
Going back to original plan, do alpha equivalence later (if needed)

proofs/core/Substitution.v
@@ -1,5 +1,6 @@
 Require Import Common.
 Require Import Syntax.
+Require Import IndTypes.
 Require Import Semantics.
 Require Import Types.
 Require Import Typing.
@@ -7,10 +8,6 @@ Require Import Denotational.
 
 Set Bullet Behavior "Strict Subproofs".
 
-(*Here we define a function to rename bound variables to unique
-  values such that terms and formulas have no duplicate bound
-  variables and no clashes between free and bound variable names.
-  This makes many transformations easier.*)
 
 (*First, some functions we need*)
 
@@ -100,9 +97,797 @@ Proof.
     + rewrite skipn_length, <- H. lia.
 Qed.
 
+Lemma NoDup_pat_fv (p: pattern) : NoDup (pat_fv p).
+Proof.
+  induction p; simpl; try constructor; auto.
+  - constructor.
+  - apply big_union_nodup.
+  - apply union_nodup; auto.
+  - apply union_nodup; auto. constructor; auto. constructor.
+Qed.
+
+(*Some tactics that will be useful:*)
+
+(*Solve trivial/repeated goals and simplify*)
+Ltac len_tac :=
+repeat match goal with
+| |- context [length (firstn ?n ?l)] => rewrite firstn_length
+| |- context [length (skipn ?n ?l)] => rewrite skipn_length
+| H: length ?l = ?x |- context [length ?l] => rewrite H
+| |- context [length (?x ++ ?y)] => rewrite app_length
+end; try lia.
+
+(*Deal with In (firstn) and similar goals*)
+(*TODO*)
+Ltac in_tac :=
+  repeat match goal with
+  | |- In (nth ?i ?l ?x) ?l =>
+    apply nth_In
+  | H: In ?x (firstn ?n ?l) |- _ => apply In_firstn in H
+  | H: In ?x (skipn ?n ?l) |- _ => apply In_skipn in H
+  | |- In ?x (map ?g ?l) => rewrite in_map_iff
+  | |- In ?x (?l1 ++ ?l2) => rewrite in_app_iff
+  | |- In ?x ?l1 \/ In ?x ?l2 => solve[left; in_tac] + solve[right; in_tac]
+  end; auto.
+
+Ltac wf_tac :=
+  repeat(
+  assumption +
+  solve[len_tac] +
+  solve[lia] +
+  solve[in_tac] +
+  match goal with
+  | |- context [map snd (combine ?l1 ?l2)] =>
+    rewrite map_snd_combine
+  | |- context [map fst (combine ?l1 ?l2)] =>
+    rewrite map_fst_combine
+  | |- NoDup (firstn ?n ?l) => apply NoDup_firstn
+  | |- NoDup (skipn ?n ?l) => apply NoDup_skipn
+  | |- NoDup (nth ?i (split_lens ?a ?b) ?d) =>
+    apply split_lens_nodup
+  | |- context [length (map ?f ?x)] => rewrite map_length
+  | |- context [length (split_lens ?l1 ?l2)] =>
+    rewrite split_lens_length
+  | |- context [length (firstn ?n ?l)] => rewrite firstn_length
+  | |- context [length (skipn ?n ?l)] => rewrite skipn_length
+  | |- In (nth ?i ?l ?x) ?l =>
+    apply nth_In
+  | |- context [length (nth ?l (split_lens ?a ?b) ?d)] =>
+    rewrite split_lens_ith
+  | |- context [length (map2 ?f ?l1 ?l2)] =>
+    rewrite map2_length
+  | |- ?i < length ?l -> ?P => intros
+  | |- context [Nat.min ?x ?x] =>
+    rewrite Nat.min_id
+  (*TODO: this is hacky*)
+  | |- context [nth ?i (map ?f ?l) ?d] =>
+    (rewrite map_nth_inbound with(d2:=tm_d)) ||
+    (rewrite map_nth_inbound with (d2:=(Pwild, tm_d))) ||
+    (rewrite map_nth_inbound with (d2:=(Pwild, Ftrue))) ||
+    (rewrite map_nth_inbound with (d2:=Pwild))
+  (*Deal with some "In" goals - TODO improve*)
+  | H: In ?x (firstn ?n ?l) |- In ?x ?l => apply In_firstn in H
+  | H: In ?x (skipn ?n ?l) |- In ?x ?l => apply In_skipn in H
+  | H: In ?x (firstn ?n ?l1) |- In ?x ?l2 => apply In_firstn in H
+  (*A special case*)
+  | |- NoDup (pat_fv ?p) => apply NoDup_pat_fv
+  | |- context [concat (split_lens ?l1 ?l2)] =>
+    rewrite <- split_lens_concat
+  | |- In ?x (map ?g ?l) => rewrite in_map_iff
+  | |- exists y, ?f y = ?f ?x /\ ?P => exists x; split
+  (*Solve the sum length goal*)
+  | H: length ?l = length (concat (map ?f ?l1)) |-
+    sum (map ?g ?l1) = length ?l => rewrite length_concat in H;
+    rewrite H; f_equal; rewrite map_map; apply map_ext
+  | H: length (?x :: ?l) = ?n |- _ => simpl in H
+  | H: ?x = length (?l1 ++ ?l2) |- _ => rewrite app_length in H
+  end); auto; try lia. 
+
+
+Ltac simpl_set_goal :=
+  repeat match goal with
+  (*remove*)
+  | H: In ?x (remove ?e ?y ?l) |- _ => rewrite in_remove_iff in H
+  | |- context [ In ?x (remove ?e ?y ?l)] => rewrite in_remove_iff
+  (*big_union*)
+  | H: In ?x (big_union ?e ?f ?l) |- _ => rewrite <- big_union_elts in H
+  | |- context [ In ?x (big_union ?e ?f ?l)] => rewrite <- big_union_elts
+  (*union*)
+  | H: In ?x (union ?e ?l1 ?l2) |- _ => rewrite union_elts in H
+  | |- context [ In ?x (union ?e ?l1 ?l2)] => rewrite union_elts
+  (*cons - TODO do without simpl*)
+  | H: In ?x (?y :: ?t) |-_ => simpl in H
+  | |- context [In ?x (?y :: ?t)] => simpl
+  (*remove \/ False from In goals*)
+  | H: ?P \/ False |- _ => rewrite or_false_r in H
+  | |- context [ ?P \/ False] => rewrite or_false_r
+  (*remove_all*)
+  | H: In ?x (remove_all ?e ?l1 ?l2) |- _ => rewrite <- remove_all_elts in H
+  | |- context [In ?x (remove_all ?e ?l1 ?l2)] => rewrite <- remove_all_elts
+  end.
+
+Ltac simpl_set :=
+  simpl_set_goal;
+  repeat match goal with
+  | H: ~ In ?x (remove_all ?e ?l1 ?l2) |- _ => revert H; simpl_set_goal; intros
+  | H: ~ In ?x (union ?e ?l1 ?l2) |- _ => revert H; simpl_set_goal; intros
+  | H: ~ In ?x (big_union ?e ?f ?l) |- _ => revert H; simpl_set_goal; intros
+  | H: ~ In ?x (remove ?e ?y ?l) |- _ => revert H; simpl_set_goal; intros
+  end.
+
+Ltac destruct_all :=
+  repeat match goal with
+  | H: ?P /\ ?Q |- _ => destruct H
+  | H: exists x, ?P |- _ => destruct H
+  | H: ?P \/ ?Q |- _ => destruct H
+  end; subst.
+
+Ltac simpl_destruct_set :=
+  repeat (progress (simpl_set; destruct_all)).
+
+Ltac triv :=
+  let inner := split_all; auto; 
+  match goal with
+  | |- ~ ?P => let C := fresh in intro C; subst; contradiction
+  end
+  in
+  try solve[inner];
+  match goal with
+  | |- ?P \/ ?Q => solve[left; inner] + solve[right; inner]
+  end.
+
+Ltac not_or name :=
+  repeat match goal with 
+  | H: ~(?P \/ ?Q) |- _ => let N1 := fresh name in
+    let N2 := fresh name in
+    apply Decidable.not_or in H;
+    
+    destruct H as [N1 N2]
+  end.
+
+Ltac case_in :=
+  repeat match goal with
+  | |- context [if in_bool ?e ?x ?l then ?y else ?z] => 
+    destruct (in_bool_spec e x l)
+  end.
+
+(*First, general and useful results about substitution*)
+
+(*Substitution for patterns - needed for bound variable
+  substitution, not free var subs like [sub_t] and [sub_f]*)
+Fixpoint sub_p (x y: vsymbol) (p: pattern) :=
+  match p with
+  | Pvar v =>
+    Pvar (if vsymbol_eq_dec v x then y else v)
+  | Pwild => Pwild
+  | Por p1 p2 => Por (sub_p x y p1) (sub_p x y p2)
+  | Pbind p1 v =>
+    Pbind (sub_p x y p1) (if vsymbol_eq_dec v x then y else v)
+  | Pconstr f tys pats =>
+    Pconstr f tys (map (sub_p x y) pats)
+  end.
+
+(*Substitute multiple vars according to map*)
+Definition sub_mult {A: Type} (sub: vsymbol -> vsymbol -> A -> A) 
+  (l: list (vsymbol * string)) (x: A) : A :=
+  fold_right (fun x acc => sub (fst x) ((snd x), snd (fst x)) acc) x l.
+
+(*Substitute multiple vars in pattern according to map*)
+Definition sub_ps : list (vsymbol * string) -> pattern -> pattern:=
+  sub_mult sub_p.
+  
+(*Substitute multiple vars in term according to map*)
+Definition sub_ts: list (vsymbol * string) -> term -> term:=
+  sub_mult sub_t.
+
+(*Substitite multiple vars in formula according to map*)
+Definition sub_fs: list (vsymbol * string) -> formula -> formula :=
+  sub_mult sub_f.
+
+(*We need a lot of results about how substition affects free
+  variables*)
+
+(*A few easy results about sub_t/f and free vars:*)
+
+(*If the free var to sub is not in the term, substitution does nothing*)
+Lemma sub_notin (t: term) (f: formula) :
+  (forall (x y: vsymbol),
+    ~ In x (term_fv t) ->
+    sub_t x y t = t) /\
+    (forall (x y: vsymbol),
+    ~ In x (form_fv f) ->
+    sub_f x y f = f).
+Proof.
+  revert t f. apply term_formula_ind; simpl; auto; intros; simpl_set; not_or Hinx.
+  - destruct (vsymbol_eq_dec x v); subst; auto; contradiction.
+  - f_equal. apply list_eq_ext';
+    rewrite map_length; auto.
+    intros.
+    rewrite (map_nth_inbound) with(d2:=d); auto.
+    rewrite Forall_forall in H. apply H; wf_tac.
+    intro C. apply H0. simpl_set.  exists (nth n l1 d); split; wf_tac.
+  - rewrite H; auto.
+    destruct (vsymbol_eq_dec x v); subst; auto.
+    rewrite H0; auto.
+  - rewrite H, H0, H1; auto.
+  - rewrite H; auto. f_equal.
+    apply list_eq_ext'; rewrite map_length; auto; intros.
+    rewrite map_nth_inbound with (d2:=d); auto.
+    case_in; auto.
+    rewrite Forall_forall in H0. rewrite H0; wf_tac.
+    destruct (nth n ps d); auto.
+    intro Hinx'. apply Hinx0. exists (nth n ps d).
+    split; wf_tac. simpl_set. split; auto.
+  - destruct (vsymbol_eq_dec x v); subst; auto.
+    rewrite H; auto.
+  - f_equal. apply list_eq_ext';
+    rewrite map_length; auto.
+    intros.
+    rewrite (map_nth_inbound) with(d2:=d); auto.
+    rewrite Forall_forall in H. apply H; wf_tac.
+    intro C. apply H0.  exists (nth n tms d); split; wf_tac.
+  - destruct (vsymbol_eq_dec x v); subst; auto.
+    rewrite H; auto.
+  - rewrite H, H0; auto.
+  - rewrite H, H0; auto.
+  - rewrite H; auto.
+  - rewrite H; auto.
+    destruct (vsymbol_eq_dec x v); subst; auto.
+    rewrite H0; auto.
+  - rewrite H, H0, H1; auto.
+  - rewrite H; auto.
+    f_equal.
+    apply list_eq_ext'; rewrite map_length; auto; intros.
+    rewrite map_nth_inbound with (d2:=d); auto.
+    case_in; auto.
+    rewrite Forall_forall in H0. rewrite H0; wf_tac.
+    destruct (nth n ps d); auto.
+    intro Hinx'. apply Hinx0. exists (nth n ps d).
+    split; wf_tac. simpl_set. split; auto.
+Qed.
+
+Corollary sub_t_notin (t: term):
+  (forall (x y: vsymbol),
+    ~ In x (term_fv t) ->
+    sub_t x y t = t).
+Proof. apply sub_notin. apply Ftrue. Qed.
+
+Corollary sub_f_notin (f: formula):
+    (forall (x y: vsymbol),
+    ~ In x (form_fv f) ->
+    sub_f x y f = f).
+Proof. apply sub_notin. apply tm_d. Qed.
+
+(*If we substitute x with itself, then nothing changes*)
+Lemma sub_eq (t: term) (f: formula) :
+  (forall (x: vsymbol),
+    sub_t x x t = t) /\
+    (forall (x: vsymbol),
+    sub_f x x f = f).
+Proof.
+  revert t f; apply term_formula_ind; simpl; auto; intros.
+  - destruct (vsymbol_eq_dec x v); subst; auto.
+  - f_equal. apply list_eq_ext'; rewrite map_length; auto; intros.
+    rewrite map_nth_inbound with(d2:=d); auto.
+    rewrite Forall_forall in H; apply H; wf_tac.
+  - rewrite H. destruct (vsymbol_eq_dec x v); subst; auto.
+    rewrite H0; auto.
+  - rewrite H, H0, H1; auto.
+  - rewrite H. f_equal. apply list_eq_ext'; rewrite map_length; auto;
+    intros. rewrite map_nth_inbound with(d2:=d); auto.
+    rewrite Forall_forall in H0; rewrite H0; wf_tac.
+    case_in; auto. destruct (nth n ps d); auto.
+  - destruct (vsymbol_eq_dec x v); subst; auto. rewrite H; auto.
+  - f_equal. apply list_eq_ext'; rewrite map_length; auto; intros.
+    rewrite map_nth_inbound with(d2:=d); auto.
+    rewrite Forall_forall in H; apply H; wf_tac.
+  - destruct (vsymbol_eq_dec x v); subst; auto. rewrite H; auto.
+  - rewrite H, H0; auto.
+  - rewrite H, H0; auto.
+  - rewrite H; auto.
+  - rewrite H, H0. destruct (vsymbol_eq_dec x v); auto.
+  - rewrite H, H0, H1; auto.
+  - rewrite H. f_equal. apply list_eq_ext'; rewrite map_length; auto;
+    intros. rewrite map_nth_inbound with(d2:=d); auto.
+    rewrite Forall_forall in H0; rewrite H0; wf_tac.
+    case_in; auto. destruct (nth n ps d); auto.
+Qed.
+
+Corollary sub_t_eq (t: term):
+  (forall (x: vsymbol),
+    sub_t x x t = t).
+Proof. apply sub_eq. apply Ftrue. Qed.
+
+Corollary sub_f_eq (f: formula):
+    (forall (x: vsymbol),
+    sub_f x x f = f).
+Proof. apply sub_eq. apply tm_d. Qed.
+
+(*It is easier to prove some of the lemmas with an alternate
+  approach: define when a variable is free rather than show
+  the sets of free vars are equal:*)
+Fixpoint free_in_t (x: vsymbol) (t: term) {struct t} : bool :=
+  match t with
+  | Tconst _ => false
+  | Tvar v => vsymbol_eq_dec x v
+  | Tfun f tys tms => existsb (fun t => free_in_t x t) tms
+  | Tlet t1 v t2 =>
+    free_in_t x t1 || (negb (vsymbol_eq_dec x v) && free_in_t x t2)
+  | Tif f t1 t2 =>
+    free_in_f x f || free_in_t x t1 || free_in_t x t2
+  | Tmatch tm ty ps =>
+    free_in_t x tm ||
+    existsb (fun p => negb (in_bool vsymbol_eq_dec x (pat_fv (fst p))) &&
+      free_in_t x (snd p)) ps
+  | Teps f v => negb (vsymbol_eq_dec x v) && free_in_f x f
+  end
+with free_in_f (x: vsymbol) (f: formula) {struct f} : bool :=
+  match f with
+  | Fpred p tys tms => existsb (fun t => free_in_t x t) tms
+  | Fquant q v f1 => negb (vsymbol_eq_dec x v) && free_in_f x f1
+  | Feq ty t1 t2 => free_in_t x t1 || free_in_t x t2
+  | Fbinop b f1 f2 => free_in_f x f1 || free_in_f x f2
+  | Fnot f1 => free_in_f x f1
+  | Flet tm v f1 => free_in_t x tm || (negb (vsymbol_eq_dec x v) &&
+   free_in_f x f1)
+  | Fif f1 f2 f3 => free_in_f x f1 || free_in_f x f2 ||
+    free_in_f x f3
+  | Fmatch tm ty ps =>
+    free_in_t x tm ||
+    (existsb (fun p => negb (in_bool vsymbol_eq_dec x (pat_fv (fst p)))
+      && free_in_f x (snd p)) ps)
+  | _ => false
+  end.
+
+Ltac bool_to_prop :=
+  repeat (progress (
+  unfold is_true;
+  (*First, convert bools to props*)
+  repeat match goal with
+  | |- context [(?b && ?b1) = true] =>
+    rewrite andb_true_iff
+  | |- context [(?b1 || ?b2) = true] =>
+    rewrite orb_true_iff
+  | |- context [existsb ?f ?l = true] =>
+    rewrite existsb_exists
+  (*| |- context [negb ?b = true] =>
+    rewrite negb_true_iff*)
+  end;
+  (*Try to simplify*)
+  repeat(
+    apply or_iff_compat_l ||
+    apply and_iff_compat_l
+  );
+  (*Put the goal in a nicer form*)
+  repeat lazymatch goal with
+  | |- ?P /\ ?Q <-> ?Q /\ ?R => rewrite (and_comm P Q)
+  | |- ?P \/ ?Q <-> ?Q \/ ?R => rewrite (or_comm P Q)
+  | |- ?P /\ ?Q <-> ?R /\ ?P => rewrite (and_comm R P)
+  | |- ?P \/ ?Q <-> ?R /\ ?P => rewrite (or_comm R P)
+  | |- context [ (?P \/ ?Q) \/ ?R] => rewrite or_assoc
+  | |- ?P <-> ?P => reflexivity
+  end)).
+
+Lemma ex_in_eq {A: Type} (l: list A) (P1 P2: A -> Prop) :
+  Forall (fun x => P1 x <-> P2 x) l ->
+  (exists x, In x l /\ P1 x) <->
+  (exists x, In x l /\ P2 x).
+Proof.
+  intros. rewrite Forall_forall in H. 
+  split; intros [x [Hinx Hpx]]; exists x; split; auto;
+  apply H; auto.
+Qed.
+
+Lemma eq_sym_iff {A: Type} (x y: A):
+  x = y <-> y = x.
+Proof.
+  split; intros; subst; auto.
+Qed.
+
+Lemma dec_iff {P: Prop} {dec: {P} + { ~ P}}:
+  dec <-> P.
+Proof.
+  destruct dec; simpl; split; intros; auto. inversion H.
+Qed.
+
+Lemma dec_negb_iff {P: Prop} {dec: {P} + {~ P}}:
+  negb dec <-> ~ P.
+Proof.
+  destruct dec; simpl; split; intros; auto.
+Qed.
+
+(*This is equivalent to the other formulation*)
+(*TODO: would be easier with ssreflect*)
+Lemma free_in_spec (t: term) (f: formula) :
+  (forall x, free_in_t x t <-> In x (term_fv t)) /\
+  (forall x, free_in_f x f <-> In x (form_fv f)).
+Proof.
+  revert t f.
+  apply term_formula_ind; simpl; intros; auto; simpl_set; auto;
+  try solve[split; auto].
+  - rewrite (eq_sym_iff v x), dec_iff; reflexivity. 
+  - bool_to_prop. apply ex_in_eq.
+    eapply Forall_impl. 2: apply H. simpl; intros; auto. apply H0; auto.
+  - rewrite <- H, <- H0. bool_to_prop.
+    apply dec_negb_iff.
+  - rewrite<- H, <- H0, <- H1.
+    bool_to_prop.
+  - rewrite <- H. bool_to_prop.
+    apply ex_in_eq.
+    revert H0. rewrite !Forall_forall; intros. simpl_set.
+    bool_to_prop.
+    rewrite <- H0; wf_tac. bool_to_prop.
+    rewrite <- in_bool_dec.
+    apply dec_negb_iff.
+  - rewrite <- H; bool_to_prop.
+    apply dec_negb_iff.
+  - bool_to_prop. apply ex_in_eq.
+    eapply Forall_impl. 2: apply H. simpl; intros; auto. apply H0; auto.
+  - rewrite <- H; bool_to_prop. apply dec_negb_iff.
+  - rewrite <- H, <- H0. bool_to_prop.
+  - rewrite <- H, <- H0; bool_to_prop.
+  - rewrite <- H, <- H0; bool_to_prop.
+    apply dec_negb_iff.
+  - rewrite <- H, <- H0, <- H1; bool_to_prop.
+  - rewrite <- H. bool_to_prop.
+    apply ex_in_eq.
+    revert H0. rewrite !Forall_forall; intros. simpl_set.
+    bool_to_prop.
+    rewrite <- H0; wf_tac. bool_to_prop.
+    rewrite <- in_bool_dec.
+    apply dec_negb_iff.
+Qed.
+
+Corollary free_in_t_spec (t: term):
+(forall x, free_in_t x t <-> In x (term_fv t)).
+Proof. apply free_in_spec. apply Ftrue. Qed.
+
+Lemma free_in_t_negb (t: term):
+forall x, free_in_t x t = false <-> ~In x (term_fv t).
+Proof.
+  intros. destruct (free_in_t x t) eqn : Hfree; split; intros; auto.
+  assert (is_true (free_in_t x t)) by auto.
+  apply free_in_t_spec in H0. contradiction.
+  intro Hin. apply free_in_t_spec in Hin.
+  rewrite Hfree in Hin. inversion Hin.
+Qed.
+
+Corollary free_in_f_spec (f: formula):
+(forall x, free_in_f x f <-> In x (form_fv f)).
+Proof. apply free_in_spec. apply tm_d. Qed.
+
+Lemma free_in_f_negb (f: formula):
+forall x, free_in_f x f = false <-> ~In x (form_fv f).
+Proof.
+  intros. destruct (free_in_f x f) eqn : Hfree; split; intros; auto.
+  assert (is_true (free_in_f x f)) by auto.
+  apply free_in_f_spec in H0. contradiction.
+  intro Hin. apply free_in_f_spec in Hin.
+  rewrite Hfree in Hin. inversion Hin.
+Qed.
+
+(*Now we can reason about [free_in]*)
+
+(*3 lemmas about free vars and [sub_t]*)
+
+Ltac vsym_eq x y :=
+  destruct (vsymbol_eq_dec x y); subst; auto; try contradiction.
+
+Lemma existsb_eq {A: Type} {f1 f2: A -> bool} (l1 l2: list A):
+  length l1 = length l2 ->
+  Forall (fun x => f1 (fst x) = f2 (snd x)) (combine l1 l2) ->
+  existsb f1 l1 = existsb f2 l2.
+Proof.
+  revert l2. induction l1; simpl; intros; destruct l2; inversion H; simpl; auto.
+  inversion H0; subst.
+  simpl in H4. rewrite H4, (IHl1 l2); auto.
+Qed. 
+  
+
+(*1. For any variables which are not x or y, sub_t doesn't change anything*)
+Lemma sub_fv_diff (t: term) (f: formula):
+  (forall (x y z: vsymbol),
+    z <> x -> z <> y ->
+    free_in_t z (sub_t x y t) = free_in_t z t) /\
+  (forall (x y z: vsymbol),
+    z <> x -> z <> y ->
+    free_in_f z (sub_f x y f) = free_in_f z f).
+Proof.
+  revert t f.
+  apply term_formula_ind; simpl; auto; intros.
+  - vsym_eq x v. vsym_eq z y. vsym_eq z v.
+  - apply existsb_eq; wf_tac.
+    revert H. rewrite !Forall_forall; intros.
+    revert H2. 
+    rewrite in_combine_iff; wf_tac.
+    intros [i [Hi Hx]]. specialize (Hx tm_d tm_d); subst; simpl.
+    wf_tac.
+    apply H; wf_tac.
+  - rewrite H; auto. f_equal. f_equal.
+    vsym_eq x v.
+  - rewrite H, H0, H1; auto.
+  - rewrite H; auto. f_equal.
+    apply existsb_eq; wf_tac.
+    revert H0.
+    rewrite !Forall_forall; intros.
+    revert H3.
+    rewrite in_combine_iff; wf_tac.
+    intros [i [Hi Hx]]; specialize (Hx (Pwild, tm_d) (Pwild, tm_d)); subst; simpl.
+    wf_tac. case_in; auto.
+    simpl; rewrite H0; wf_tac.
+  - vsym_eq x v. simpl. rewrite H; auto.
+  - apply existsb_eq; wf_tac.
+    revert H. rewrite !Forall_forall; intros.
+    revert H2. 
+    rewrite in_combine_iff; wf_tac.
+    intros [i [Hi Hx]]. specialize (Hx tm_d tm_d); subst; simpl.
+    wf_tac.
+    apply H; wf_tac.
+  - vsym_eq x v; simpl; rewrite H; auto.
+  - rewrite H, H0; auto.
+  - rewrite H, H0; auto.
+  - rewrite H; auto. f_equal. f_equal.
+    vsym_eq x v.
+  - rewrite H, H0, H1; auto.
+  - rewrite H; auto. f_equal.
+    apply existsb_eq; wf_tac.
+    revert H0.
+    rewrite !Forall_forall; intros.
+    revert H3.
+    rewrite in_combine_iff; wf_tac.
+    intros [i [Hi Hx]]; specialize (Hx (Pwild, Ftrue) (Pwild, Ftrue)); subst; simpl.
+    wf_tac. case_in; auto.
+    simpl; rewrite H0; wf_tac.
+Qed.
+
+Corollary sub_t_fv_diff (t: term):
+  (forall (x y z: vsymbol),
+    z <> x -> z <> y ->
+    free_in_t z (sub_t x y t) = free_in_t z t).
+Proof. apply sub_fv_diff. apply Ftrue. Qed.
+
+Corollary sub_f_fv_diff (f:formula):
+  (forall (x y z: vsymbol),
+    z <> x -> z <> y ->
+    free_in_f z (sub_f x y f) = free_in_f z f).
+Proof. apply sub_fv_diff. apply tm_d. Qed.
+
+Lemma existsb_false {A: Type} (f: A -> bool) (l: list A):
+  (existsb f l = false) <-> Forall (fun x => f x = false) l.
+Proof.
+  induction l; simpl; split; intros; auto.
+  - rewrite orb_false_iff in H.
+    destruct_all; subst; constructor; auto.
+    apply IHl; auto.
+  - rewrite orb_false_iff. inversion H; subst.
+    split; auto. apply IHl; auto.
+Qed.
+
+(*2: If we replace x with y, x is NOT in the resulting free variables*)
+Lemma sub_fv_notin (t: term) (f: formula):
+  (forall (x y: vsymbol),
+    x <> y ->
+    free_in_t x (sub_t x y t) = false) /\
+  (forall (x y: vsymbol),
+    x <> y ->
+    free_in_f x (sub_f x y f) = false).
+Proof.
+  revert t f. apply term_formula_ind; simpl; auto; intros.
+  - vsym_eq x v. vsym_eq v y. vsym_eq x v.
+  - apply existsb_false.
+    revert H. rewrite !Forall_forall; intros.
+    revert H1. rewrite in_map_iff; intros [t [Ht Hint]]; subst.
+    apply H; auto.
+  - rewrite !orb_false_iff. split; [apply H; auto|].
+    vsym_eq x v. simpl. apply H0; auto.
+  - rewrite H, H0, H1; auto.
+  - rewrite H; simpl; auto.
+    apply existsb_false. revert H0. rewrite !Forall_forall; intros.
+    revert H2. rewrite in_map_iff; intros [p1 [Hp1 Hinp1]]; subst.
+    case_in; simpl; destruct (in_bool_spec vsymbol_eq_dec x (pat_fv (fst p1))); simpl; auto;
+    try contradiction.
+    apply H0; wf_tac.
+  - vsym_eq x v; simpl; auto. vsym_eq v v.
+    vsym_eq x v; simpl. apply H; auto.
+  - apply existsb_false.
+    revert H. rewrite !Forall_forall; intros.
+    revert H1. rewrite in_map_iff; intros [t [Ht Hint]]; subst.
+    apply H; auto.
+  - vsym_eq x v; simpl. vsym_eq v v. vsym_eq x v; simpl.
+    apply H; auto.
+  - rewrite H, H0; auto.
+  - rewrite H, H0; auto.
+  - rewrite H; auto; simpl. vsym_eq x v; simpl.
+    apply H0; auto.
+  - rewrite H, H0, H1; auto.
+  - rewrite H; simpl; auto.
+    apply existsb_false. revert H0. rewrite !Forall_forall; intros.
+    revert H2. rewrite in_map_iff; intros [p1 [Hp1 Hinp1]]; subst.
+    case_in; simpl; destruct (in_bool_spec vsymbol_eq_dec x (pat_fv (fst p1))); simpl; auto;
+    try contradiction.
+    apply H0; wf_tac.
+Qed.
+
+Corollary sub_t_fv_notin (t: term):
+  (forall (x y: vsymbol),
+    x <> y ->
+    free_in_t x (sub_t x y t) = false).
+Proof. apply sub_fv_notin. apply Ftrue. Qed.
+
+Corollary sub_f_fv_notin (f: formula):
+  (forall (x y: vsymbol),
+    x <> y ->
+    free_in_f x (sub_f x y f) = false).
+Proof. apply sub_fv_notin. apply tm_d. Qed.
+
+Lemma existsb_orb {A: Type} (f1 f2: A -> bool) (l: list A):
+  existsb f1 l || existsb f2 l =
+  existsb (fun x => f1 x || f2 x) l.
+Proof.
+  induction l; simpl; auto.
+  rewrite <- !orb_assoc. f_equal.
+  rewrite orb_comm, <- orb_assoc. f_equal.
+  rewrite orb_comm; apply IHl.
+Qed.
+
+Ltac simpl_bool :=
+  repeat (progress (simpl;
+  try rewrite !orb_assoc;
+  try rewrite !andb_assoc;
+  repeat match goal with
+  | |- context [ ?b && true] => rewrite andb_true_r
+  | |- context [?b || true] => rewrite orb_true_r
+  | |- context [?b && false] => rewrite andb_false_r
+  | |- context [?b || false] => rewrite orb_false_r
+  end)).
+
+Ltac solve_bool :=
+  simpl_bool;
+  (*Then brute force the solution*)
+  repeat 
+  (match goal with
+  | |- ?b1 && ?b2 = ?z => destruct b2
+  | |- ?b1 || ?b2 = ?z => destruct b2
+  | |- ?z = ?b1 && ?b2 => destruct b2
+  | |- ?z = ?b1 || ?b2 => destruct b2
+  end; simpl_bool; try reflexivity).
+
+
+(*3. When we substitute x with y, y is in the free variables
+  iff either y was before or x was before*)
+(*Need the Hbnd assumption for the following: in let t1 = v in t2,
+  if y =v, then y will not be in the free variables of
+  the substituted term even if x is a free variable in t2*)
+Lemma sub_fv_in (t: term) (f: formula):
+  (forall (x y: vsymbol)
+    (Hbnd: ~ In y (bnd_t t)),
+    x <> y ->
+    free_in_t y (sub_t x y t) = (free_in_t x t) || (free_in_t y t)) /\
+  (forall (x y: vsymbol)
+    (Hbnd: ~ In y (bnd_f f)),
+    x <> y ->
+    free_in_f y (sub_f x y f) = (free_in_f x f) || (free_in_f y f)).
+Proof.
+  revert t f. apply term_formula_ind; simpl; auto; intros.
+  - vsym_eq x v; simpl.
+    vsym_eq y y.
+  - rewrite existsb_orb.
+    apply existsb_eq; wf_tac.
+    revert H. rewrite !Forall_forall; intros.
+    revert H1. rewrite in_combine_iff; wf_tac.
+    intros [i [Hi Hx]]. specialize (Hx tm_d tm_d); subst; simpl.
+    wf_tac. apply H; wf_tac. intro C.
+    apply Hbnd. rewrite in_concat. exists (bnd_t (nth i l1 tm_d)); 
+    split; wf_tac.
+  - rewrite H; auto; [|intro C; apply Hbnd; right; apply in_or_app; triv]. 
+    rewrite <- !orb_assoc. f_equal.
+    rewrite !orb_andb_distrib_r.
+    vsym_eq x v.
+    rewrite H0; auto; [|intro C; apply Hbnd; right; apply in_or_app; triv].
+    vsym_eq y v. exfalso. apply Hbnd; triv.
+    simpl. solve_bool.
+  - rewrite H, H0, H1; auto;[solve_bool| | |]; intro C; apply Hbnd;
+    rewrite !in_app_iff; triv.
+  - (*match is hard case not surprisingly*)
+    rewrite H; auto; [|intro C; apply Hbnd; rewrite in_app_iff; triv].
+    simpl_bool. rewrite (orb_comm (_ || _) (free_in_t y tm)).
+    rewrite orb_assoc, (orb_comm (free_in_t y tm)).
+    rewrite <- !orb_assoc. f_equal. f_equal.
+    (*Now just have the exists goal*)
+    rewrite existsb_orb.
+    apply existsb_eq; wf_tac.
+    revert H0. rewrite !Forall_forall; intros.
+    revert H2. rewrite in_combine_iff; wf_tac; intros [i [Hi Hx]].
+    specialize (Hx (Pwild, tm_d) (Pwild, tm_d)); subst; simpl.
+    wf_tac. case_in; simpl; auto.
+    destruct (in_bool_spec vsymbol_eq_dec y (pat_fv (fst (nth i ps (Pwild, tm_d))))); simpl.
+    + (*contradiction: y not in bound vars*)
+      exfalso. apply Hbnd. rewrite in_app_iff. right.
+      rewrite in_concat. exists ((pat_fv (fst (nth i ps (Pwild, tm_d))))
+      ++ (bnd_t (snd (nth i ps (Pwild, tm_d))))).
+      split; wf_tac. exists (nth i ps (Pwild, tm_d)). split; wf_tac.
+    + rewrite H0; wf_tac. intro C.
+      apply Hbnd. rewrite in_app_iff. right. 
+      rewrite in_concat. exists ((pat_fv (fst (nth i ps (Pwild, tm_d))))
+      ++ (bnd_t (snd (nth i ps (Pwild, tm_d))))).
+      split; wf_tac. exists (nth i ps (Pwild, tm_d)). split; wf_tac.
+  - vsym_eq x v; simpl.
+    vsym_eq y v; simpl.
+    + exfalso; apply Hbnd; triv.
+    + rewrite H; auto.
+  - rewrite existsb_orb.
+    apply existsb_eq; wf_tac.
+    revert H. rewrite !Forall_forall; intros.
+    revert H1. rewrite in_combine_iff; wf_tac.
+    intros [i [Hi Hx]]. specialize (Hx tm_d tm_d); subst; simpl.
+    wf_tac. apply H; wf_tac. intro C.
+    apply Hbnd. rewrite in_concat. exists (bnd_t (nth i tms tm_d)); 
+    split; wf_tac.
+  - vsym_eq x v; simpl.
+    vsym_eq y v; simpl.
+    + exfalso; apply Hbnd; triv.
+    + rewrite H; auto.
+  - rewrite H, H0; auto; [solve_bool | |]; intro C; apply Hbnd;
+    rewrite in_app_iff; triv.
+  - rewrite H, H0; auto; [solve_bool | |]; intro C; apply Hbnd;
+    rewrite in_app_iff; triv.
+  - rewrite H; auto; [|intro C; apply Hbnd; right; apply in_or_app; triv]. 
+    rewrite <- !orb_assoc. f_equal.
+    rewrite !orb_andb_distrib_r.
+    vsym_eq x v.
+    rewrite H0; auto; [|intro C; apply Hbnd; right; apply in_or_app; triv].
+    vsym_eq y v. exfalso. apply Hbnd; triv.
+    simpl. solve_bool.
+  - rewrite H, H0, H1; auto;[solve_bool | | |]; intro C;
+    apply Hbnd; rewrite !in_app_iff; triv.
+  - rewrite H; auto; [|intro C; apply Hbnd; rewrite in_app_iff; triv].
+    simpl_bool. rewrite (orb_comm (_ || _) (free_in_t y tm)).
+    rewrite orb_assoc, (orb_comm (free_in_t y tm)).
+    rewrite <- !orb_assoc. f_equal. f_equal.
+    (*Now just have the exists goal*)
+    rewrite existsb_orb.
+    apply existsb_eq; wf_tac.
+    revert H0. rewrite !Forall_forall; intros.
+    revert H2. rewrite in_combine_iff; wf_tac; intros [i [Hi Hx]].
+    specialize (Hx (Pwild, Ftrue) (Pwild, Ftrue)); subst; simpl.
+    wf_tac. case_in; simpl; auto.
+    destruct (in_bool_spec vsymbol_eq_dec y (pat_fv (fst (nth i ps (Pwild, Ftrue))))); simpl.
+    + (*contradiction: y not in bound vars*)
+      exfalso. apply Hbnd. rewrite in_app_iff. right.
+      rewrite in_concat. exists ((pat_fv (fst (nth i ps (Pwild, Ftrue))))
+      ++ (bnd_f (snd (nth i ps (Pwild, Ftrue))))).
+      split; wf_tac. exists (nth i ps (Pwild, Ftrue)). split; wf_tac.
+    + rewrite H0; wf_tac. intro C.
+      apply Hbnd. rewrite in_app_iff. right. 
+      rewrite in_concat. exists ((pat_fv (fst (nth i ps (Pwild, Ftrue))))
+      ++ (bnd_f (snd (nth i ps (Pwild, Ftrue))))).
+      split; wf_tac. exists (nth i ps (Pwild, Ftrue)). split; wf_tac.
+Qed. 
+
+Corollary sub_t_fv_in (t: term):
+  (forall (x y: vsymbol)
+    (Hbnd: ~ In y (bnd_t t)),
+    x <> y ->
+    free_in_t y (sub_t x y t) = (free_in_t x t) || (free_in_t y t)). 
+Proof. apply sub_fv_in. apply Ftrue. Qed.
+
+Corollary sub_f_fv_in (f: formula):
+  (forall (x y: vsymbol)
+    (Hbnd: ~ In y (bnd_f f)),
+    x <> y ->
+    free_in_f y (sub_f x y f) = (free_in_f x f) || (free_in_f y f)).
+Proof. apply sub_fv_in. apply tm_d. Qed.
+
+(*Now we want to define a function to rename bound variables to unique
+  values such that terms and formulas have no duplicate bound
+  variables and no clashes between free and bound variable names.
+  This makes many transformations easier.*)
+
 Section Sub.
 Context {sigma: sig} {gamma: context} (gamma_valid: valid_context sigma gamma).
 
+(*
+  
 
 (*Alpha substitute for patterns only in the given term/formula*)
 (*Here, we need to keep the dependencies between pattern variables
@@ -143,7 +928,7 @@ Context {sigma: sig} {gamma: context} (gamma_valid: valid_context sigma gamma).
       | nil => (nil, y)
       end) pats x) in
     (Pconstr f tys (fst t), (snd t))
-    end.
+    end.*)
 (*Proving this correct will not be too fun, but let's see*)
 
 Fixpoint alpha_t_aux (t: term) (l: list string) {struct t} : term :=
@@ -186,8 +971,8 @@ Fixpoint alpha_t_aux (t: term) (l: list string) {struct t} : term :=
         let p_sz := length (pat_fv (fst x)) in
         let (l1, l2) := split strs p_sz in
         let t2 := alpha_t_aux (snd x) l2 in
-        alpha_p_aux sub_t (fst x) t2  (combine (pat_fv (fst x)) l1)
-        ) ps l_split)
+        let vars := combine (pat_fv (fst x)) l1 in
+        (sub_ps vars (fst x), sub_ts vars t2)) ps l_split)
   | Teps f v =>
     match l with
     | nil => t
@@ -255,8 +1040,8 @@ with alpha_f_aux (f: formula) (l: list string) {struct f} : formula :=
         let p_sz := length (pat_fv (fst x)) in
         let (l1, l2) := split strs p_sz in
         let f2 := alpha_f_aux (snd x) l2 in
-        alpha_p_aux sub_f (fst x) f2  (combine (pat_fv (fst x)) l1)
-        ) ps l_split)
+        let vars := combine (pat_fv (fst x)) l1 in
+        (sub_ps vars (fst x), sub_fs vars f2)) ps l_split)
   | _ => f (*No other bound/recursive cases*)
   end.
 (*Prove correctness: 3 lemmas
@@ -265,15 +1050,9 @@ with alpha_f_aux (f: formula) (l: list string) {struct f} : formula :=
   3. has same "shape" (and corollaries: ind form, positive, etc)*)
 
 
-Lemma NoDup_pat_fv (p: pattern) : NoDup (pat_fv p).
-Proof.
-  induction p; simpl; try constructor; auto.
-  - constructor.
-  - apply big_union_nodup.
-  - apply union_nodup; auto.
-  - apply union_nodup; auto. constructor; auto. constructor.
-Qed.
 
+
+(*
 (*TODO: see if we need*)
 Lemma alpha_p_aux_wf_aux_gen {A: Type} (p: pattern) 
   (sub: vsymbol -> vsymbol -> A -> A) :
@@ -483,82 +1262,146 @@ Proof.
     rewrite IHps; auto.
   - destruct (get_assoc_list vsymbol_eq_dec l v); simpl; auto.
     rewrite bnd_sub_f; auto.
+Qed.*)
+
+(*TODO: move this stuff probably*)
+
+(*First, sub_ts does not change bound vars*)
+Lemma bnd_sub_ts l t :
+  bnd_t (sub_ts l t) = bnd_t t.
+Proof.
+  induction l; simpl; auto.
+  rewrite bnd_sub_t; auto.
 Qed.
 
+(*Need free vars of [sub_ps]*)
+
+(*Let's do similar to [sub_t]*)
+Fixpoint free_in_p (x: vsymbol) (p: pattern) : bool :=
+  match p with
+  | Pvar v => vsymbol_eq_dec x v
+  | Pwild => false
+  | Pbind p1 v => vsymbol_eq_dec x v || free_in_p x p1
+  | Por p1 p2 => free_in_p x p1 || free_in_p x p2
+  | Pconstr f tys ps =>
+    existsb (fun p => free_in_p x p) ps
+  end.
+
+Lemma free_in_p_spec (p: pattern) (x: vsymbol):
+  free_in_p x p <-> In x (pat_fv p).
+Proof.
+  induction p; simpl; simpl_set; auto; try solve[split; auto].
+  - rewrite (eq_sym_iff v x), dec_iff; reflexivity.
+  - bool_to_prop. apply ex_in_eq.
+    apply H.
+  - bool_to_prop. rewrite IHp1, IHp2; reflexivity.
+  - bool_to_prop. rewrite IHp. bool_to_prop.
+    rewrite (eq_sym_iff v x).
+    vsym_eq x v; simpl; split; auto; intros; inversion H.
+Qed.
+
+
+(*we only need a subset of the results, because we work with
+  vars guaranteed to be in [pat_fv p] and different than existing
+  vars*)
+
+
+(*1. For any variables which are not x or y, sub_p doesn't change anything*)
+Lemma sub_p_fv_diff (p: pattern):
+  forall (x y z: vsymbol),
+  z <> x -> z <> y ->
+  free_in_p z (sub_p x y p) = free_in_p z p.
+Proof.
+  induction p; simpl; intros; auto.
+  - vsym_eq v x. vsym_eq z y. vsym_eq z x.
+  - apply existsb_eq; wf_tac.
+    revert H. rewrite !Forall_forall; intros.
+    revert H2. rewrite in_combine_iff; wf_tac.
+    intros [i [Hi Hx]]. specialize (Hx Pwild Pwild); subst; simpl.
+    wf_tac. apply H; wf_tac.
+  - rewrite IHp1, IHp2; wf_tac.
+  - rewrite IHp; wf_tac. vsym_eq v x.
+    vsym_eq z y. vsym_eq z x.
+Qed. 
+
+(*2: If we replace x with y, x is NOT in the resulting free variables*)
+Lemma sub_p_fv_notin (p: pattern) :
+  forall (x y: vsymbol),
+  x <> y ->
+  free_in_p x (sub_p x y p) = false.
+Proof.
+  intros; induction p; simpl; auto.
+  - vsym_eq v x. vsym_eq x y. vsym_eq x v.
+  - apply existsb_false.
+    revert H0. rewrite !Forall_forall; intros.
+    revert H1. rewrite in_map_iff; intros [t [Ht Hint]]; subst.
+    apply H0; auto.
+  - rewrite IHp1, IHp2. auto.
+  - rewrite IHp. simpl_bool.
+    vsym_eq v x. vsym_eq x y. vsym_eq x v.
+Qed.
+
+(*3. When we substitute x with y, y is in the free variables
+  iff either y was before or x was before*)
+Lemma sub_p_fv_in (p: pattern):
+  forall (x y: vsymbol),
+  x <> y ->
+  free_in_p y (sub_p x y p) = (free_in_p x p) || (free_in_p y p).
+Proof.
+  intros; induction p; simpl; auto.
+  - vsym_eq x v; simpl. vsym_eq v v. vsym_eq y y. vsym_eq v x.
+  - rewrite existsb_orb. apply existsb_eq; wf_tac.
+    revert H0. rewrite !Forall_forall; intros.
+    revert H1; rewrite in_combine_iff; wf_tac.
+    intros [i [Hi Hx]]. specialize (Hx Pwild Pwild); subst; simpl.
+    wf_tac. apply H0; wf_tac.
+  - rewrite IHp1, IHp2; solve_bool.
+  - rewrite IHp. vsym_eq v x.
+    + vsym_eq y y. vsym_eq x x.
+    + vsym_eq x v. vsym_eq y v. solve_bool; auto.
+Qed.
+
+(*TODO: prove result for [sub_ps] that we end up with only
+  the domain of the list (basically what we need i think)*)
+
+(*TODO: may need stronger lemma later - look at sub_t and sub_f 
+  for this*)
+  (*hmm look at sub_t tbh*)
+Lemma pat_fv_sub_p x y p:
+  In x (pat_fv p) ->
+  x <> y ->
+  forall v,
+  In v (pat_fv (sub_p x y p)) <-> v = y \/ (v <> x /\ In v (pat_fv p)).
+Proof.
+  induction p; simpl; simpl_set; intros; subst; simpl_set.
+  - destruct (vsymbol_eq_dec x x); try contradiction.
+    split; intros; destruct_all; auto. contradiction.
+  - split; intros.
+    + destruct_all.
+      rewrite in_map_iff in H2. destruct_all.
+      rewrite Forall_forall in H. apply H in H3; auto.
+
+
+    split; intros; destruct_all; try split; auto.
+    + right. split; auto. intro; subst.
+
+
+
+Lemma pat_fv_sub_p x y p :
+  x <> y ->
+  forall v,
+  In v (pat_fv (sub_p x y p)) <->
+  (v <> x /\ (In x (pat_fv p) /\ v = y) \/ (In v (pat_fv p))).
+Proof.
+  intros. induction p; simpl; simpl_set.
+  - destruct (vsymbol_eq_dec v0 x); subst; split; intros.
+    + subst. triv.
+    + destruct_all; auto.
+    destruct_all.
+  subst. split; intros. left; auto. destruct H. subst; split; intros; 
+    destruct_all; subst; auto.
+
 (*TODO: add to this*)
-(*Solve trivial/repeated goals and simplify*)
-Ltac len_tac :=
-repeat match goal with
-| |- context [length (firstn ?n ?l)] => rewrite firstn_length
-| |- context [length (skipn ?n ?l)] => rewrite skipn_length
-| H: length ?l = ?x |- context [length ?l] => rewrite H
-| |- context [length (?x ++ ?y)] => rewrite app_length
-end; try lia.
-
-(*Deal with In (firstn) and similar goals*)
-(*TODO*)
-Ltac in_tac :=
-  repeat match goal with
-  | |- In (nth ?i ?l ?x) ?l =>
-    apply nth_In
-  | H: In ?x (firstn ?n ?l) |- _ => apply In_firstn in H
-  | H: In ?x (skipn ?n ?l) |- _ => apply In_skipn in H
-  | |- In ?x (map ?g ?l) => rewrite in_map_iff
-  | |- In ?x (?l1 ++ ?l2) => rewrite in_app_iff
-  | |- In ?x ?l1 \/ In ?x ?l2 => solve[left; in_tac] + solve[right; in_tac]
-  end; auto.
-
-Ltac wf_tac :=
-  repeat(
-  assumption +
-  solve[len_tac] +
-  solve[lia] +
-  solve[in_tac] +
-  match goal with
-  | |- context [map snd (combine ?l1 ?l2)] =>
-    rewrite map_snd_combine
-  | |- context [map fst (combine ?l1 ?l2)] =>
-    rewrite map_fst_combine
-  | |- NoDup (firstn ?n ?l) => apply NoDup_firstn
-  | |- NoDup (skipn ?n ?l) => apply NoDup_skipn
-  | |- NoDup (nth ?i (split_lens ?a ?b) ?d) =>
-    apply split_lens_nodup
-  | |- context [length (map ?f ?x)] => rewrite map_length
-  | |- context [length (split_lens ?l1 ?l2)] =>
-    rewrite split_lens_length
-  | |- context [length (firstn ?n ?l)] => rewrite firstn_length
-  | |- context [length (skipn ?n ?l)] => rewrite skipn_length
-  | |- In (nth ?i ?l ?x) ?l =>
-    apply nth_In
-  | |- context [length (nth ?l (split_lens ?a ?b) ?d)] =>
-    rewrite split_lens_ith
-  | |- context [length (map2 ?f ?l1 ?l2)] =>
-    rewrite map2_length
-  | |- ?i < length ?l -> ?P => intros
-  | |- context [Nat.min ?x ?x] =>
-    rewrite Nat.min_id
-  (*TODO: this is hacky*)
-  | |- context [nth ?i (map ?f ?l) ?d] =>
-    (rewrite map_nth_inbound with(d2:=tm_d)) ||
-    (rewrite map_nth_inbound with (d2:=(Pwild, tm_d))) ||
-    (rewrite map_nth_inbound with (d2:=(Pwild, Ftrue)))
-  (*Deal with some "In" goals - TODO improve*)
-  | H: In ?x (firstn ?n ?l) |- In ?x ?l => apply In_firstn in H
-  | H: In ?x (skipn ?n ?l) |- In ?x ?l => apply In_skipn in H
-  | H: In ?x (firstn ?n ?l1) |- In ?x ?l2 => apply In_firstn in H
-  (*A special case*)
-  | |- NoDup (pat_fv ?p) => apply NoDup_pat_fv
-  | |- context [concat (split_lens ?l1 ?l2)] =>
-    rewrite <- split_lens_concat
-  | |- In ?x (map ?g ?l) => rewrite in_map_iff
-  | |- exists y, ?f y = ?f ?x /\ ?P => exists x; split
-  (*Solve the sum length goal*)
-  | H: length ?l = length (concat (map ?f ?l1)) |-
-    sum (map ?g ?l1) = length ?l => rewrite length_concat in H;
-    rewrite H; f_equal; rewrite map_map; apply map_ext
-  | H: length (?x :: ?l) = ?n |- _ => simpl in H
-  | H: ?x = length (?l1 ++ ?l2) |- _ => rewrite app_length in H
-  end); auto; try lia. 
 
 Lemma alpha_aux_wf_aux (t: term) (f: formula) :
   (forall (l: list string),
@@ -675,11 +1518,11 @@ Proof.
           destruct Hinx as [i [Hi Hpt1]].
           rewrite NoDup_app_iff'.
           split_all; subst; wf_tac.
-          ++ rewrite alpha_p_aux_bnd_t_eq.
+          ++ simpl. rewrite bnd_sub_ts.
             rewrite Forall_forall in H0.
             apply H0; auto; wf_tac.
-          ++ intros x.
-            rewrite alpha_p_aux_bnd_t_eq.
+          ++ intros x. simpl.
+            rewrite bnd_sub_ts. 
             intros [Hinx1 Hinx2].
             (*Need this a lot even though it's ugly*)
             apply alpha_p_aux_wf_aux in Hinx1; wf_tac.
@@ -1333,669 +2176,9 @@ Proof.
   apply alpha_aux_valid. apply tm_d.
 Qed.
 
-(*Part 2.5: We need to know that this substitution does not
+(*Part 2.5 We need to know that this substitution does not
   change the free variables. This is very hard to show, particularly
   due to the patterns and their dependencies*)
-
-(*Some tactics that will be useful:*)
-
-Ltac simpl_set_goal :=
-  repeat match goal with
-  (*remove*)
-  | H: In ?x (remove ?e ?y ?l) |- _ => rewrite in_remove_iff in H
-  | |- context [ In ?x (remove ?e ?y ?l)] => rewrite in_remove_iff
-  (*big_union*)
-  | H: In ?x (big_union ?e ?f ?l) |- _ => rewrite <- big_union_elts in H
-  | |- context [ In ?x (big_union ?e ?f ?l)] => rewrite <- big_union_elts
-  (*union*)
-  | H: In ?x (union ?e ?l1 ?l2) |- _ => rewrite union_elts in H
-  | |- context [ In ?x (union ?e ?l1 ?l2)] => rewrite union_elts
-  (*cons - TODO do without simpl*)
-  | H: In ?x (?y :: ?t) |-_ => simpl in H
-  | |- context [In ?x (?y :: ?t)] => simpl
-  (*remove \/ False from In goals*)
-  | H: ?P \/ False |- _ => rewrite or_false_r in H
-  | |- context [ ?P \/ False] => rewrite or_false_r
-  (*remove_all*)
-  | H: In ?x (remove_all ?e ?l1 ?l2) |- _ => rewrite <- remove_all_elts in H
-  | |- context [In ?x (remove_all ?e ?l1 ?l2)] => rewrite <- remove_all_elts
-  end.
-
-Ltac simpl_set :=
-  simpl_set_goal;
-  repeat match goal with
-  | H: ~ In ?x (remove_all ?e ?l1 ?l2) |- _ => revert H; simpl_set_goal; intros
-  | H: ~ In ?x (union ?e ?l1 ?l2) |- _ => revert H; simpl_set_goal; intros
-  | H: ~ In ?x (big_union ?e ?f ?l) |- _ => revert H; simpl_set_goal; intros
-  | H: ~ In ?x (remove ?e ?y ?l) |- _ => revert H; simpl_set_goal; intros
-  end.
-
-Ltac destruct_all :=
-  repeat match goal with
-  | H: ?P /\ ?Q |- _ => destruct H
-  | H: exists x, ?P |- _ => destruct H
-  | H: ?P \/ ?Q |- _ => destruct H
-  end; subst.
-
-Ltac simpl_destruct_set :=
-  repeat (progress (simpl_set; destruct_all)).
-
-Ltac triv :=
-  let inner := split_all; auto; 
-  match goal with
-  | |- ~ ?P => let C := fresh in intro C; subst; contradiction
-  end
-  in
-  try solve[inner];
-  match goal with
-  | |- ?P \/ ?Q => solve[left; inner] + solve[right; inner]
-  end.
-
-Ltac not_or name :=
-  repeat match goal with 
-  | H: ~(?P \/ ?Q) |- _ => let N1 := fresh name in
-    let N2 := fresh name in
-    apply Decidable.not_or in H;
-    
-    destruct H as [N1 N2]
-  end.
-
-Ltac case_in :=
-  repeat match goal with
-  | |- context [if in_bool ?e ?x ?l then ?y else ?z] => 
-    destruct (in_bool_spec e x l)
-  end.
-
-(*A few easy results about sub_t/f and free vars:*)
-
-(*If the free var to sub is not in the term, substitution does nothing*)
-Lemma sub_notin (t: term) (f: formula) :
-  (forall (x y: vsymbol),
-    ~ In x (term_fv t) ->
-    sub_t x y t = t) /\
-    (forall (x y: vsymbol),
-    ~ In x (form_fv f) ->
-    sub_f x y f = f).
-Proof.
-  revert t f. apply term_formula_ind; simpl; auto; intros; simpl_set; not_or Hinx.
-  - destruct (vsymbol_eq_dec x v); subst; auto; contradiction.
-  - f_equal. apply list_eq_ext';
-    rewrite map_length; auto.
-    intros.
-    rewrite (map_nth_inbound) with(d2:=d); auto.
-    rewrite Forall_forall in H. apply H; wf_tac.
-    intro C. apply H0. simpl_set.  exists (nth n l1 d); split; wf_tac.
-  - rewrite H; auto.
-    destruct (vsymbol_eq_dec x v); subst; auto.
-    rewrite H0; auto.
-  - rewrite H, H0, H1; auto.
-  - rewrite H; auto. f_equal.
-    apply list_eq_ext'; rewrite map_length; auto; intros.
-    rewrite map_nth_inbound with (d2:=d); auto.
-    case_in; auto.
-    rewrite Forall_forall in H0. rewrite H0; wf_tac.
-    destruct (nth n ps d); auto.
-    intro Hinx'. apply Hinx0. exists (nth n ps d).
-    split; wf_tac. simpl_set. split; auto.
-  - destruct (vsymbol_eq_dec x v); subst; auto.
-    rewrite H; auto.
-  - f_equal. apply list_eq_ext';
-    rewrite map_length; auto.
-    intros.
-    rewrite (map_nth_inbound) with(d2:=d); auto.
-    rewrite Forall_forall in H. apply H; wf_tac.
-    intro C. apply H0.  exists (nth n tms d); split; wf_tac.
-  - destruct (vsymbol_eq_dec x v); subst; auto.
-    rewrite H; auto.
-  - rewrite H, H0; auto.
-  - rewrite H, H0; auto.
-  - rewrite H; auto.
-  - rewrite H; auto.
-    destruct (vsymbol_eq_dec x v); subst; auto.
-    rewrite H0; auto.
-  - rewrite H, H0, H1; auto.
-  - rewrite H; auto.
-    f_equal.
-    apply list_eq_ext'; rewrite map_length; auto; intros.
-    rewrite map_nth_inbound with (d2:=d); auto.
-    case_in; auto.
-    rewrite Forall_forall in H0. rewrite H0; wf_tac.
-    destruct (nth n ps d); auto.
-    intro Hinx'. apply Hinx0. exists (nth n ps d).
-    split; wf_tac. simpl_set. split; auto.
-Qed.
-
-Corollary sub_t_notin (t: term):
-  (forall (x y: vsymbol),
-    ~ In x (term_fv t) ->
-    sub_t x y t = t).
-Proof. apply sub_notin. apply Ftrue. Qed.
-
-Corollary sub_f_notin (f: formula):
-    (forall (x y: vsymbol),
-    ~ In x (form_fv f) ->
-    sub_f x y f = f).
-Proof. apply sub_notin. apply tm_d. Qed.
-
-(*If we substitute x with itself, then nothing changes*)
-Lemma sub_eq (t: term) (f: formula) :
-  (forall (x: vsymbol),
-    sub_t x x t = t) /\
-    (forall (x: vsymbol),
-    sub_f x x f = f).
-Proof.
-  revert t f; apply term_formula_ind; simpl; auto; intros.
-  - destruct (vsymbol_eq_dec x v); subst; auto.
-  - f_equal. apply list_eq_ext'; rewrite map_length; auto; intros.
-    rewrite map_nth_inbound with(d2:=d); auto.
-    rewrite Forall_forall in H; apply H; wf_tac.
-  - rewrite H. destruct (vsymbol_eq_dec x v); subst; auto.
-    rewrite H0; auto.
-  - rewrite H, H0, H1; auto.
-  - rewrite H. f_equal. apply list_eq_ext'; rewrite map_length; auto;
-    intros. rewrite map_nth_inbound with(d2:=d); auto.
-    rewrite Forall_forall in H0; rewrite H0; wf_tac.
-    case_in; auto. destruct (nth n ps d); auto.
-  - destruct (vsymbol_eq_dec x v); subst; auto. rewrite H; auto.
-  - f_equal. apply list_eq_ext'; rewrite map_length; auto; intros.
-    rewrite map_nth_inbound with(d2:=d); auto.
-    rewrite Forall_forall in H; apply H; wf_tac.
-  - destruct (vsymbol_eq_dec x v); subst; auto. rewrite H; auto.
-  - rewrite H, H0; auto.
-  - rewrite H, H0; auto.
-  - rewrite H; auto.
-  - rewrite H, H0. destruct (vsymbol_eq_dec x v); auto.
-  - rewrite H, H0, H1; auto.
-  - rewrite H. f_equal. apply list_eq_ext'; rewrite map_length; auto;
-    intros. rewrite map_nth_inbound with(d2:=d); auto.
-    rewrite Forall_forall in H0; rewrite H0; wf_tac.
-    case_in; auto. destruct (nth n ps d); auto.
-Qed.
-
-Corollary sub_t_eq (t: term):
-  (forall (x: vsymbol),
-    sub_t x x t = t).
-Proof. apply sub_eq. apply Ftrue. Qed.
-
-Corollary sub_f_eq (f: formula):
-    (forall (x: vsymbol),
-    sub_f x x f = f).
-Proof. apply sub_eq. apply tm_d. Qed.
-
-(*It is easier to prove some of the lemmas with an alternate
-  approach: define when a variable is free rather than show
-  the sets of free vars are equal:*)
-Fixpoint free_in_t (x: vsymbol) (t: term) {struct t} : bool :=
-  match t with
-  | Tconst _ => false
-  | Tvar v => vsymbol_eq_dec x v
-  | Tfun f tys tms => existsb (fun t => free_in_t x t) tms
-  | Tlet t1 v t2 =>
-    free_in_t x t1 || (negb (vsymbol_eq_dec x v) && free_in_t x t2)
-  | Tif f t1 t2 =>
-    free_in_f x f || free_in_t x t1 || free_in_t x t2
-  | Tmatch tm ty ps =>
-    free_in_t x tm ||
-    existsb (fun p => negb (in_bool vsymbol_eq_dec x (pat_fv (fst p))) &&
-      free_in_t x (snd p)) ps
-  | Teps f v => negb (vsymbol_eq_dec x v) && free_in_f x f
-  end
-with free_in_f (x: vsymbol) (f: formula) {struct f} : bool :=
-  match f with
-  | Fpred p tys tms => existsb (fun t => free_in_t x t) tms
-  | Fquant q v f1 => negb (vsymbol_eq_dec x v) && free_in_f x f1
-  | Feq ty t1 t2 => free_in_t x t1 || free_in_t x t2
-  | Fbinop b f1 f2 => free_in_f x f1 || free_in_f x f2
-  | Fnot f1 => free_in_f x f1
-  | Flet tm v f1 => free_in_t x tm || (negb (vsymbol_eq_dec x v) &&
-   free_in_f x f1)
-  | Fif f1 f2 f3 => free_in_f x f1 || free_in_f x f2 ||
-    free_in_f x f3
-  | Fmatch tm ty ps =>
-    free_in_t x tm ||
-    (existsb (fun p => negb (in_bool vsymbol_eq_dec x (pat_fv (fst p)))
-      && free_in_f x (snd p)) ps)
-  | _ => false
-  end.
-
-Ltac bool_to_prop :=
-  repeat (progress (
-  unfold is_true;
-  (*First, convert bools to props*)
-  repeat match goal with
-  | |- context [(?b && ?b1) = true] =>
-    rewrite andb_true_iff
-  | |- context [(?b1 || ?b2) = true] =>
-    rewrite orb_true_iff
-  | |- context [existsb ?f ?l = true] =>
-    rewrite existsb_exists
-  (*| |- context [negb ?b = true] =>
-    rewrite negb_true_iff*)
-  end;
-  (*Try to simplify*)
-  repeat(
-    apply or_iff_compat_l ||
-    apply and_iff_compat_l
-  );
-  (*Put the goal in a nicer form*)
-  repeat lazymatch goal with
-  | |- ?P /\ ?Q <-> ?Q /\ ?R => rewrite (and_comm P Q)
-  | |- ?P \/ ?Q <-> ?Q \/ ?R => rewrite (or_comm P Q)
-  | |- ?P /\ ?Q <-> ?R /\ ?P => rewrite (and_comm R P)
-  | |- ?P \/ ?Q <-> ?R /\ ?P => rewrite (or_comm R P)
-  | |- context [ (?P \/ ?Q) \/ ?R] => rewrite or_assoc
-  | |- ?P <-> ?P => reflexivity
-  end)).
-
-Lemma ex_in_eq {A: Type} (l: list A) (P1 P2: A -> Prop) :
-  Forall (fun x => P1 x <-> P2 x) l ->
-  (exists x, In x l /\ P1 x) <->
-  (exists x, In x l /\ P2 x).
-Proof.
-  intros. rewrite Forall_forall in H. 
-  split; intros [x [Hinx Hpx]]; exists x; split; auto;
-  apply H; auto.
-Qed.
-
-Lemma eq_sym_iff {A: Type} (x y: A):
-  x = y <-> y = x.
-Proof.
-  split; intros; subst; auto.
-Qed.
-
-Lemma dec_iff {P: Prop} {dec: {P} + { ~ P}}:
-  dec <-> P.
-Proof.
-  destruct dec; simpl; split; intros; auto. inversion H.
-Qed.
-
-Lemma dec_negb_iff {P: Prop} {dec: {P} + {~ P}}:
-  negb dec <-> ~ P.
-Proof.
-  destruct dec; simpl; split; intros; auto.
-Qed.
-
-(*This is equivalent to the other formulation*)
-(*TODO: would be easier with ssreflect*)
-Lemma free_in_spec (t: term) (f: formula) :
-  (forall x, free_in_t x t <-> In x (term_fv t)) /\
-  (forall x, free_in_f x f <-> In x (form_fv f)).
-Proof.
-  revert t f.
-  apply term_formula_ind; simpl; intros; auto; simpl_set; auto;
-  try solve[split; auto].
-  - rewrite (eq_sym_iff v x), dec_iff; reflexivity. 
-  - bool_to_prop. apply ex_in_eq.
-    eapply Forall_impl. 2: apply H. simpl; intros; auto. apply H0; auto.
-  - rewrite <- H, <- H0. bool_to_prop.
-    apply dec_negb_iff.
-  - rewrite<- H, <- H0, <- H1.
-    bool_to_prop.
-  - rewrite <- H. bool_to_prop.
-    apply ex_in_eq.
-    revert H0. rewrite !Forall_forall; intros. simpl_set.
-    bool_to_prop.
-    rewrite <- H0; wf_tac. bool_to_prop.
-    rewrite <- in_bool_dec.
-    apply dec_negb_iff.
-  - rewrite <- H; bool_to_prop.
-    apply dec_negb_iff.
-  - bool_to_prop. apply ex_in_eq.
-    eapply Forall_impl. 2: apply H. simpl; intros; auto. apply H0; auto.
-  - rewrite <- H; bool_to_prop. apply dec_negb_iff.
-  - rewrite <- H, <- H0. bool_to_prop.
-  - rewrite <- H, <- H0; bool_to_prop.
-  - rewrite <- H, <- H0; bool_to_prop.
-    apply dec_negb_iff.
-  - rewrite <- H, <- H0, <- H1; bool_to_prop.
-  - rewrite <- H. bool_to_prop.
-    apply ex_in_eq.
-    revert H0. rewrite !Forall_forall; intros. simpl_set.
-    bool_to_prop.
-    rewrite <- H0; wf_tac. bool_to_prop.
-    rewrite <- in_bool_dec.
-    apply dec_negb_iff.
-Qed.
-
-Corollary free_in_t_spec (t: term):
-(forall x, free_in_t x t <-> In x (term_fv t)).
-Proof. apply free_in_spec. apply Ftrue. Qed.
-
-Lemma free_in_t_negb (t: term):
-forall x, free_in_t x t = false <-> ~In x (term_fv t).
-Proof.
-  intros. destruct (free_in_t x t) eqn : Hfree; split; intros; auto.
-  assert (is_true (free_in_t x t)) by auto.
-  apply free_in_t_spec in H0. contradiction.
-  intro Hin. apply free_in_t_spec in Hin.
-  rewrite Hfree in Hin. inversion Hin.
-Qed.
-
-Corollary free_in_f_spec (f: formula):
-(forall x, free_in_f x f <-> In x (form_fv f)).
-Proof. apply free_in_spec. apply tm_d. Qed.
-
-Lemma free_in_f_negb (f: formula):
-forall x, free_in_f x f = false <-> ~In x (form_fv f).
-Proof.
-  intros. destruct (free_in_f x f) eqn : Hfree; split; intros; auto.
-  assert (is_true (free_in_f x f)) by auto.
-  apply free_in_f_spec in H0. contradiction.
-  intro Hin. apply free_in_f_spec in Hin.
-  rewrite Hfree in Hin. inversion Hin.
-Qed.
-
-(*Now we can reason about [free_in]*)
-
-(*3 lemmas about free vars and [sub_t]*)
-
-Ltac vsym_eq x y :=
-  destruct (vsymbol_eq_dec x y); subst; auto; try contradiction.
-
-Lemma existsb_eq {A: Type} {f1 f2: A -> bool} (l1 l2: list A):
-  length l1 = length l2 ->
-  Forall (fun x => f1 (fst x) = f2 (snd x)) (combine l1 l2) ->
-  existsb f1 l1 = existsb f2 l2.
-Proof.
-  revert l2. induction l1; simpl; intros; destruct l2; inversion H; simpl; auto.
-  inversion H0; subst.
-  simpl in H4. rewrite H4, (IHl1 l2); auto.
-Qed. 
-  
-
-(*1. For any variables which are not x or y, sub_t doesn't change anything*)
-Lemma sub_fv_diff (t: term) (f: formula):
-  (forall (x y z: vsymbol),
-    z <> x -> z <> y ->
-    free_in_t z (sub_t x y t) = free_in_t z t) /\
-  (forall (x y z: vsymbol),
-    z <> x -> z <> y ->
-    free_in_f z (sub_f x y f) = free_in_f z f).
-Proof.
-  revert t f.
-  apply term_formula_ind; simpl; auto; intros.
-  - vsym_eq x v. vsym_eq z y. vsym_eq z v.
-  - apply existsb_eq; wf_tac.
-    revert H. rewrite !Forall_forall; intros.
-    revert H2. 
-    rewrite in_combine_iff; wf_tac.
-    intros [i [Hi Hx]]. specialize (Hx tm_d tm_d); subst; simpl.
-    wf_tac.
-    apply H; wf_tac.
-  - rewrite H; auto. f_equal. f_equal.
-    vsym_eq x v.
-  - rewrite H, H0, H1; auto.
-  - rewrite H; auto. f_equal.
-    apply existsb_eq; wf_tac.
-    revert H0.
-    rewrite !Forall_forall; intros.
-    revert H3.
-    rewrite in_combine_iff; wf_tac.
-    intros [i [Hi Hx]]; specialize (Hx (Pwild, tm_d) (Pwild, tm_d)); subst; simpl.
-    wf_tac. case_in; auto.
-    simpl; rewrite H0; wf_tac.
-  - vsym_eq x v. simpl. rewrite H; auto.
-  - apply existsb_eq; wf_tac.
-    revert H. rewrite !Forall_forall; intros.
-    revert H2. 
-    rewrite in_combine_iff; wf_tac.
-    intros [i [Hi Hx]]. specialize (Hx tm_d tm_d); subst; simpl.
-    wf_tac.
-    apply H; wf_tac.
-  - vsym_eq x v; simpl; rewrite H; auto.
-  - rewrite H, H0; auto.
-  - rewrite H, H0; auto.
-  - rewrite H; auto. f_equal. f_equal.
-    vsym_eq x v.
-  - rewrite H, H0, H1; auto.
-  - rewrite H; auto. f_equal.
-    apply existsb_eq; wf_tac.
-    revert H0.
-    rewrite !Forall_forall; intros.
-    revert H3.
-    rewrite in_combine_iff; wf_tac.
-    intros [i [Hi Hx]]; specialize (Hx (Pwild, Ftrue) (Pwild, Ftrue)); subst; simpl.
-    wf_tac. case_in; auto.
-    simpl; rewrite H0; wf_tac.
-Qed.
-
-Corollary sub_t_fv_diff (t: term):
-  (forall (x y z: vsymbol),
-    z <> x -> z <> y ->
-    free_in_t z (sub_t x y t) = free_in_t z t).
-Proof. apply sub_fv_diff. apply Ftrue. Qed.
-
-Corollary sub_f_fv_diff (f:formula):
-  (forall (x y z: vsymbol),
-    z <> x -> z <> y ->
-    free_in_f z (sub_f x y f) = free_in_f z f).
-Proof. apply sub_fv_diff. apply tm_d. Qed.
-
-Lemma existsb_false {A: Type} (f: A -> bool) (l: list A):
-  (existsb f l = false) <-> Forall (fun x => f x = false) l.
-Proof.
-  induction l; simpl; split; intros; auto.
-  - rewrite orb_false_iff in H.
-    destruct_all; subst; constructor; auto.
-    apply IHl; auto.
-  - rewrite orb_false_iff. inversion H; subst.
-    split; auto. apply IHl; auto.
-Qed.
-
-(*2: If we replace x with y, x is NOT in the resulting free variables*)
-Lemma sub_fv_notin (t: term) (f: formula):
-  (forall (x y: vsymbol),
-    x <> y ->
-    free_in_t x (sub_t x y t) = false) /\
-  (forall (x y: vsymbol),
-    x <> y ->
-    free_in_f x (sub_f x y f) = false).
-Proof.
-  revert t f. apply term_formula_ind; simpl; auto; intros.
-  - vsym_eq x v. vsym_eq v y. vsym_eq x v.
-  - apply existsb_false.
-    revert H. rewrite !Forall_forall; intros.
-    revert H1. rewrite in_map_iff; intros [t [Ht Hint]]; subst.
-    apply H; auto.
-  - rewrite !orb_false_iff. split; [apply H; auto|].
-    vsym_eq x v. simpl. apply H0; auto.
-  - rewrite H, H0, H1; auto.
-  - rewrite H; simpl; auto.
-    apply existsb_false. revert H0. rewrite !Forall_forall; intros.
-    revert H2. rewrite in_map_iff; intros [p1 [Hp1 Hinp1]]; subst.
-    case_in; simpl; destruct (in_bool_spec vsymbol_eq_dec x (pat_fv (fst p1))); simpl; auto;
-    try contradiction.
-    apply H0; wf_tac.
-  - vsym_eq x v; simpl; auto. vsym_eq v v.
-    vsym_eq x v; simpl. apply H; auto.
-  - apply existsb_false.
-    revert H. rewrite !Forall_forall; intros.
-    revert H1. rewrite in_map_iff; intros [t [Ht Hint]]; subst.
-    apply H; auto.
-  - vsym_eq x v; simpl. vsym_eq v v. vsym_eq x v; simpl.
-    apply H; auto.
-  - rewrite H, H0; auto.
-  - rewrite H, H0; auto.
-  - rewrite H; auto; simpl. vsym_eq x v; simpl.
-    apply H0; auto.
-  - rewrite H, H0, H1; auto.
-  - rewrite H; simpl; auto.
-    apply existsb_false. revert H0. rewrite !Forall_forall; intros.
-    revert H2. rewrite in_map_iff; intros [p1 [Hp1 Hinp1]]; subst.
-    case_in; simpl; destruct (in_bool_spec vsymbol_eq_dec x (pat_fv (fst p1))); simpl; auto;
-    try contradiction.
-    apply H0; wf_tac.
-Qed.
-
-Corollary sub_t_fv_notin (t: term):
-  (forall (x y: vsymbol),
-    x <> y ->
-    free_in_t x (sub_t x y t) = false).
-Proof. apply sub_fv_notin. apply Ftrue. Qed.
-
-Corollary sub_f_fv_notin (f: formula):
-  (forall (x y: vsymbol),
-    x <> y ->
-    free_in_f x (sub_f x y f) = false).
-Proof. apply sub_fv_notin. apply tm_d. Qed.
-
-Lemma existsb_orb {A: Type} (f1 f2: A -> bool) (l: list A):
-  existsb f1 l || existsb f2 l =
-  existsb (fun x => f1 x || f2 x) l.
-Proof.
-  induction l; simpl; auto.
-  rewrite <- !orb_assoc. f_equal.
-  rewrite orb_comm, <- orb_assoc. f_equal.
-  rewrite orb_comm; apply IHl.
-Qed.
-
-Ltac simpl_bool :=
-  repeat (progress (simpl;
-  try rewrite !orb_assoc;
-  try rewrite !andb_assoc;
-  repeat match goal with
-  | |- context [ ?b && true] => rewrite andb_true_r
-  | |- context [?b || true] => rewrite orb_true_r
-  | |- context [?b && false] => rewrite andb_false_r
-  | |- context [?b || false] => rewrite orb_false_r
-  end)).
-
-Ltac solve_bool :=
-  simpl_bool;
-  (*Then brute force the solution*)
-  repeat 
-  (match goal with
-  | |- ?b1 && ?b2 = ?z => destruct b2
-  | |- ?b1 || ?b2 = ?z => destruct b2
-  | |- ?z = ?b1 && ?b2 => destruct b2
-  | |- ?z = ?b1 || ?b2 => destruct b2
-  end; simpl_bool; try reflexivity).
-
-
-(*3. When we substitute x with y, y is in the free variables
-  iff either y was before or x was before*)
-(*Need the Hbnd assumption for the following: in let t1 = v in t2,
-  if y =v, then y will not be in the free variables of
-  the substituted term even if x is a free variable in t2*)
-Lemma sub_fv_in (t: term) (f: formula):
-  (forall (x y: vsymbol)
-    (Hbnd: ~ In y (bnd_t t)),
-    x <> y ->
-    free_in_t y (sub_t x y t) = (free_in_t x t) || (free_in_t y t)) /\
-  (forall (x y: vsymbol)
-    (Hbnd: ~ In y (bnd_f f)),
-    x <> y ->
-    free_in_f y (sub_f x y f) = (free_in_f x f) || (free_in_f y f)).
-Proof.
-  revert t f. apply term_formula_ind; simpl; auto; intros.
-  - vsym_eq x v; simpl.
-    vsym_eq y y.
-  - rewrite existsb_orb.
-    apply existsb_eq; wf_tac.
-    revert H. rewrite !Forall_forall; intros.
-    revert H1. rewrite in_combine_iff; wf_tac.
-    intros [i [Hi Hx]]. specialize (Hx tm_d tm_d); subst; simpl.
-    wf_tac. apply H; wf_tac. intro C.
-    apply Hbnd. rewrite in_concat. exists (bnd_t (nth i l1 tm_d)); 
-    split; wf_tac.
-  - rewrite H; auto; [|intro C; apply Hbnd; right; apply in_or_app; triv]. 
-    rewrite <- !orb_assoc. f_equal.
-    rewrite !orb_andb_distrib_r.
-    vsym_eq x v.
-    rewrite H0; auto; [|intro C; apply Hbnd; right; apply in_or_app; triv].
-    vsym_eq y v. exfalso. apply Hbnd; triv.
-    simpl. solve_bool.
-  - rewrite H, H0, H1; auto;[solve_bool| | |]; intro C; apply Hbnd;
-    rewrite !in_app_iff; triv.
-  - (*match is hard case not surprisingly*)
-    rewrite H; auto; [|intro C; apply Hbnd; rewrite in_app_iff; triv].
-    simpl_bool. rewrite (orb_comm (_ || _) (free_in_t y tm)).
-    rewrite orb_assoc, (orb_comm (free_in_t y tm)).
-    rewrite <- !orb_assoc. f_equal. f_equal.
-    (*Now just have the exists goal*)
-    rewrite existsb_orb.
-    apply existsb_eq; wf_tac.
-    revert H0. rewrite !Forall_forall; intros.
-    revert H2. rewrite in_combine_iff; wf_tac; intros [i [Hi Hx]].
-    specialize (Hx (Pwild, tm_d) (Pwild, tm_d)); subst; simpl.
-    wf_tac. case_in; simpl; auto.
-    destruct (in_bool_spec vsymbol_eq_dec y (pat_fv (fst (nth i ps (Pwild, tm_d))))); simpl.
-    + (*contradiction: y not in bound vars*)
-      exfalso. apply Hbnd. rewrite in_app_iff. right.
-      rewrite in_concat. exists ((pat_fv (fst (nth i ps (Pwild, tm_d))))
-      ++ (bnd_t (snd (nth i ps (Pwild, tm_d))))).
-      split; wf_tac. exists (nth i ps (Pwild, tm_d)). split; wf_tac.
-    + rewrite H0; wf_tac. intro C.
-      apply Hbnd. rewrite in_app_iff. right. 
-      rewrite in_concat. exists ((pat_fv (fst (nth i ps (Pwild, tm_d))))
-      ++ (bnd_t (snd (nth i ps (Pwild, tm_d))))).
-      split; wf_tac. exists (nth i ps (Pwild, tm_d)). split; wf_tac.
-  - vsym_eq x v; simpl.
-    vsym_eq y v; simpl.
-    + exfalso; apply Hbnd; triv.
-    + rewrite H; auto.
-  - rewrite existsb_orb.
-    apply existsb_eq; wf_tac.
-    revert H. rewrite !Forall_forall; intros.
-    revert H1. rewrite in_combine_iff; wf_tac.
-    intros [i [Hi Hx]]. specialize (Hx tm_d tm_d); subst; simpl.
-    wf_tac. apply H; wf_tac. intro C.
-    apply Hbnd. rewrite in_concat. exists (bnd_t (nth i tms tm_d)); 
-    split; wf_tac.
-  - vsym_eq x v; simpl.
-    vsym_eq y v; simpl.
-    + exfalso; apply Hbnd; triv.
-    + rewrite H; auto.
-  - rewrite H, H0; auto; [solve_bool | |]; intro C; apply Hbnd;
-    rewrite in_app_iff; triv.
-  - rewrite H, H0; auto; [solve_bool | |]; intro C; apply Hbnd;
-    rewrite in_app_iff; triv.
-  - rewrite H; auto; [|intro C; apply Hbnd; right; apply in_or_app; triv]. 
-    rewrite <- !orb_assoc. f_equal.
-    rewrite !orb_andb_distrib_r.
-    vsym_eq x v.
-    rewrite H0; auto; [|intro C; apply Hbnd; right; apply in_or_app; triv].
-    vsym_eq y v. exfalso. apply Hbnd; triv.
-    simpl. solve_bool.
-  - rewrite H, H0, H1; auto;[solve_bool | | |]; intro C;
-    apply Hbnd; rewrite !in_app_iff; triv.
-  - rewrite H; auto; [|intro C; apply Hbnd; rewrite in_app_iff; triv].
-    simpl_bool. rewrite (orb_comm (_ || _) (free_in_t y tm)).
-    rewrite orb_assoc, (orb_comm (free_in_t y tm)).
-    rewrite <- !orb_assoc. f_equal. f_equal.
-    (*Now just have the exists goal*)
-    rewrite existsb_orb.
-    apply existsb_eq; wf_tac.
-    revert H0. rewrite !Forall_forall; intros.
-    revert H2. rewrite in_combine_iff; wf_tac; intros [i [Hi Hx]].
-    specialize (Hx (Pwild, Ftrue) (Pwild, Ftrue)); subst; simpl.
-    wf_tac. case_in; simpl; auto.
-    destruct (in_bool_spec vsymbol_eq_dec y (pat_fv (fst (nth i ps (Pwild, Ftrue))))); simpl.
-    + (*contradiction: y not in bound vars*)
-      exfalso. apply Hbnd. rewrite in_app_iff. right.
-      rewrite in_concat. exists ((pat_fv (fst (nth i ps (Pwild, Ftrue))))
-      ++ (bnd_f (snd (nth i ps (Pwild, Ftrue))))).
-      split; wf_tac. exists (nth i ps (Pwild, Ftrue)). split; wf_tac.
-    + rewrite H0; wf_tac. intro C.
-      apply Hbnd. rewrite in_app_iff. right. 
-      rewrite in_concat. exists ((pat_fv (fst (nth i ps (Pwild, Ftrue))))
-      ++ (bnd_f (snd (nth i ps (Pwild, Ftrue))))).
-      split; wf_tac. exists (nth i ps (Pwild, Ftrue)). split; wf_tac.
-Qed. 
-
-Corollary sub_t_fv_in (t: term):
-  (forall (x y: vsymbol)
-    (Hbnd: ~ In y (bnd_t t)),
-    x <> y ->
-    free_in_t y (sub_t x y t) = (free_in_t x t) || (free_in_t y t)). 
-Proof. apply sub_fv_in. apply Ftrue. Qed.
-
-Corollary sub_f_fv_in (f: formula):
-  (forall (x y: vsymbol)
-    (Hbnd: ~ In y (bnd_f f)),
-    x <> y ->
-    free_in_f y (sub_f x y f) = (free_in_f x f) || (free_in_f y f)).
-Proof. apply sub_fv_in. apply tm_d. Qed.
 
 (*Analagous lemmas for term/formula in [alpha_p_aux]. These 
   are much harder*)
@@ -2809,6 +2992,9 @@ Context {pd: pi_dom} (all_unif: forall m, mut_in_ctx m gamma -> IndTypes.uniform
 Notation term_rep := (term_rep gamma_valid pd all_unif vt pf).
 Notation formula_rep := (formula_rep gamma_valid pd all_unif vt pf).
 
+(*
+
+TODO: maybe alpha equiv later
 
 (*Let's try this*)
 Print term.
@@ -3197,6 +3383,8 @@ Definition vs_d : vsymbol := (a, vty_int).
     really we want to say: for any pair not in the map, our valuations
     are the same (right)*)
   (*need to think about how valuation is changing*)
+(*NOTE: need to change in var case to check both sides, or else
+  \y.x and \x.x are considered equivalent*)
 Lemma alpha_equiv_equiv (t: term) (f: formula) :
   (forall (t2: term) (vars: list (vsymbol * vsymbol)) 
   (v1 v2: val_vars pd vt) (ty: vty)
@@ -3207,12 +3395,9 @@ Lemma alpha_equiv_equiv (t: term) (f: formula) :
     In (x, y) vars ->
     v1 x = (dom_cast _ (f_equal _ (eq_sym Heq))
     (v2 y)))
-  (Hvals2: forall x y,
-    ~ In (x, y) vars ->
+  (Hvals2: forall x,
+    (~In x (map fst vars) /\ ~ In x (map snd vars)) ->
     v1 x = v2 x)
-  (Hvals3: forall x y,
-  ~ In (x, y) vars ->
-  v1 y = v2 y)
   (Hvars1: NoDup (map fst vars))
   (Hvars2: NoDup (map snd vars)),
   term_rep v1 t ty Hty =
@@ -3226,12 +3411,9 @@ Lemma alpha_equiv_equiv (t: term) (f: formula) :
     In (x, y) vars ->
     v1 x = (dom_cast _ (f_equal _ (eq_sym Heq))
     (v2 y)))
-  (Hvals2: forall x y,
-    ~ In (x, y) vars ->
+  (Hvals2: forall x,
+    (~In x (map fst vars) /\ ~ In x (map snd vars)) ->
     v1 x = v2 x)
-  (Hvals3: forall x y,
-  ~ In (x, y) vars ->
-  v1 y = v2 y)
   (Hvars1: NoDup (map fst vars))
   (Hvars2: NoDup (map snd vars)),
   formula_rep v1 f Hval =
@@ -3259,8 +3441,7 @@ Proof.
     + apply get_assoc_list_none in Ha.
       erewrite term_fv_agree. apply term_rep_irrel. simpl.
       intros. destruct H as [Heq | []]; subst.
-      apply (Hvals2 x vs_d); auto.
-      intro C. apply Ha. wf_tac. exists (x, vs_d). wf_tac.
+      apply Hvals2.
   - destruct t2; try solve[inversion Heq]. 
     revert Heq. bool_to_prop.
     intros [[[Hfeq Hleneq] Htyeq] Hall]. repeat simpl_sumbool.
@@ -3366,7 +3547,123 @@ Proof.
     Search all_dec.
     destruct Heq.
 
+*)
 
+
+(*our lemma should say something like:
+suppose that [match_val_single] on (t, p) gives Some l
+then [match_val_single] on t, (fst (alpha_p_aux sub_t p _ l')) gives
+Some l2 where
+(x, y) is in l iff exists x' such that (x, x') in l' and (x', y) is in l2
+(might also need, NoDup (map fst)) for each)
+
+and then say: if gives None, then other gives None also (maybe prove first)
+
+then from this, need to prove that [extend_val_with_list] is equivalent
+in each case, because we do all the substitutions for the term
+(need to reason about (snd (alpha_p_aux)))
+
+*)
+Require Import Coq.Logic.Eqdep_dec.
+
+Ltac simpl_proj :=
+  simpl projT1; simpl projT2; simpl proj1_sig; simpl proj2_sig.
+
+Lemma match_val_single_alpha_p_none {A: Type} (vv: val_vars pd vt) {ty: vty}
+(Hval Hval2: valid_type sigma ty)
+(d: IndTypes.domain (dom_aux pd) (v_subst (v_typevar vt) ty))
+(p: pattern)
+(sub: vsymbol -> vsymbol -> A -> A)
+(tm: A)
+(vars: list (vsymbol * string)) :
+match_val_single gamma_valid pd all_unif vt ty Hval d p = None ->
+match_val_single gamma_valid pd all_unif vt ty Hval2 d
+  (fst (alpha_p_aux sub p tm vars)) = None.
+Proof.
+  induction p.
+  - simpl. destruct (vty_eq_dec (snd v) ty); simpl; subst.
+    intro C; inversion C. intros _.
+    destruct (get_assoc_list vsymbol_eq_dec vars v) eqn : Ha; simpl;
+    destruct (vty_eq_dec (snd v) ty); subst; auto; contradiction.
+  - (*hard case*)
+    simpl alpha_p_aux. simpl fst.
+    unfold match_val_single; repeat fold (match_val_single gamma_valid).
+    (*The hard case: need lots of generalization for dependent types
+    and need nested induction*) 
+    generalize dependent (is_sort_adt_spec gamma_valid (v_subst (v_typevar vt) ty)).
+    generalize dependent ((@adt_srts_length_eq _ _ gamma_valid vt ty)).
+    generalize dependent (@adts_srts_valid _ _ gamma_valid vt ty).
+    destruct (is_sort_adt (v_subst (v_typevar vt) ty)) eqn : Hisadt; [|solve[auto]].
+    intros Hsrtsvalid Hsrtslen Hadtspec.
+    destruct p as [[[m adt] ts] srts].
+    destruct (Hadtspec m adt ts srts eq_refl) as 
+      [Hvaleq [Hinmut [Hincts Htseq]]].
+    assert (Hlenpeq : (Hsrtslen m adt ts srts eq_refl Hval) =
+    (Hsrtslen m adt ts srts eq_refl Hval2)). {
+      apply UIP_dec. apply Nat.eq_dec.
+    }
+    rewrite <- !Hlenpeq.
+    destruct (funsym_eq_dec
+    (projT1
+      (find_constr_rep gamma_valid m Hincts srts
+          (Hsrtslen m adt ts srts eq_refl Hval) (dom_aux pd) adt
+          Hinmut (adts pd m srts) (all_unif m Hincts)
+          (scast (adts pd m srts adt Hinmut)
+            (dom_cast (dom_aux pd) Hvaleq d)))) f);[|solve[auto]].
+    clear Hlenpeq.
+    (*Need nested induction: simplify first*)
+    generalize dependent (find_constr_rep gamma_valid m Hincts srts
+    (Hsrtslen m adt ts srts eq_refl Hval) 
+    (dom_aux pd) adt Hinmut (adts pd m srts)
+    (all_unif m Hincts)
+    (scast (adts pd m srts adt Hinmut)
+      (dom_cast (dom_aux pd) Hvaleq d))).
+    intros constr. destruct constr as [f' Hf'].
+    simpl_proj.  intros Hf; subst.
+    generalize dependent ((Hsrtsvalid m adt (adt_name adt) srts f eq_refl Hval (fst (proj1_sig Hf')))).
+    generalize dependent ((Hsrtsvalid m adt (adt_name adt) srts f eq_refl Hval2 (fst (proj1_sig Hf')))).
+    destruct Hf'. simpl_proj. clear e.
+    destruct x. generalize dependent a.
+    generalize dependent ps. 
+    generalize dependent ((funsym_sigma_args f srts)).
+    induction l; intros. 
+    + destruct ps. inversion H0. reflexivity.
+    + revert H0. destruct ps. reflexivity. simpl fst. simpl snd. 
+      cbv iota. cbv beta. cbv match. (*simpl freezes*)
+      repeat match goal with 
+      |- (match ?p with |Some l => ?x | None => ?y end) = ?z -> ?q =>
+        let Hp := fresh "Hmatch" in 
+        destruct p eqn: Hp end.
+      all: try solve[intro C; inversion C].
+      * intros _. eapply IHl in Hmatch0. apply Hmatch0.
+      subst.
+      apply IHl.
+      apply in_app_or in H1. destruct H1.
+      * inversion H; subst.
+        apply H3 with(x:=x) (t:=t) in Hmatch; auto.
+      * apply IHl with(x:=x) (t:=t) in Hmatch0; auto.
+        inversion H; subst. auto.
+  - simpl; auto.
+  - simpl. destruct (match_val_single gamma_valid pd all_unif vt ty Hval d p1) eqn : Hm1;
+    [intro C; inversion C|].
+    rewrite IHp1; auto.
+  - simpl. destruct (match_val_single gamma_valid pd all_unif vt ty Hval d p) eqn : Hm.
+    + destruct (vty_eq_dec (snd v) ty); subst; auto; [intro C; inversion C|].
+      intros _. destruct (get_assoc_list vsymbol_eq_dec vars v) eqn : Ha; simpl.
+      * destruct (match_val_single gamma_valid pd all_unif vt ty Hval2 d
+        (fst (alpha_p_aux sub p tm vars))); auto.
+        destruct (vty_eq_dec (snd v) ty); subst; auto; contradiction.
+      * destruct (match_val_single gamma_valid pd all_unif vt ty Hval2 d p); auto.
+        destruct (vty_eq_dec (snd v) ty); subst; auto; contradiction.
+    + intros _. destruct (get_assoc_list vsymbol_eq_dec vars v) eqn : Ha; simpl.
+      * rewrite IHp; auto.
+      * rewrite match_val_single_irrel with (Hval2:=Hval).
+        rewrite Hm; auto.
+(*TODO: constr case*)
+      
+      [intros C; inversion C|]; auto.
+      ; simpl simpl.
+    + auto.
 
 
 Lemma alpha_aux_rep (t: term) (f: formula) :
@@ -3470,10 +3767,112 @@ Proof.
     generalize dependent (proj1 (ty_match_inv (has_type_eq eq_refl Hty2))).
     generalize dependent (proj2 (ty_match_inv (has_type_eq eq_refl Hty2))).
     induction ps; simpl; intros;[reflexivity |].
-    destruct a.
+    destruct a. simpl.
+    revert f. simpl.
+    destruct (alpha_p_aux sub_t p
+    (alpha_t_aux t1
+       (skipn (Datatypes.length (pat_fv p))
+          (firstn
+             (Datatypes.length (pat_fv p) + Datatypes.length (bnd_t t1))
+             (skipn (Datatypes.length (bnd_t tm)) l))))
+    (combine (pat_fv p)
+       (firstn (Datatypes.length (pat_fv p))
+          (firstn
+             (Datatypes.length (pat_fv p) + Datatypes.length (bnd_t t1))
+             (skipn (Datatypes.length (bnd_t tm)) l))))) eqn : Hap.
+    simpl. intros.
+    rewrite H with(l:=(firstn (Datatypes.length (bnd_t tm)) l))
+      (Hty2:=t); wf_tac.
     (*Need to know that [match_val_single] is same - or at least
       the relationship here - separate lemma?*)
-    + reflexivity.
+    Check match_val_single.
+
+    match_val_single gamma_valid pd all_unif vt v
+    (has_type_valid gamma_valid tm v t0)
+    (term_rep vv (alpha_t_aux tm (firstn (Datatypes.length (bnd_t tm)) l)) v
+       t) p
+
+    match_val_single gamma_valid pd all_unif vt v
+    (has_type_valid gamma_valid
+      (alpha_t_aux tm (firstn (Datatypes.length (bnd_t tm)) l)) v t)
+    (term_rep vv (alpha_t_aux tm (firstn (Datatypes.length (bnd_t tm)) l)) v
+      t) p0
+
+(*think: pattern (fst part) unaffected by term arg*)
+
+(*our lemma should say something like:
+suppose that [match_val_single] on (t, p) gives Some l
+then [match_val_single] on t, (fst (alpha_p_aux sub_t p _ l')) gives
+Some l2 where
+(x, y) is in l iff exists x' such that (x, x') in l' and (x', y) is in l2
+(might also need, NoDup (map fst)) for each)
+
+and then say: if gives None, then other gives None also (maybe prove first)
+
+then from this, need to prove that [extend_val_with_list] is equivalent
+in each case, because we do all the substitutions for the term
+(need to reason about (snd (alpha_p_aux)))
+
+*)
+
+    p0 = fst (alpha_p_aux sub_t p
+    (alpha_t_aux t1
+       (skipn (Datatypes.length (pat_fv p))
+          (firstn
+             (Datatypes.length (pat_fv p) + Datatypes.length (bnd_t t1))
+             (skipn (Datatypes.length (bnd_t tm)) l))))
+    (combine (pat_fv p)
+       (firstn (Datatypes.length (pat_fv p))
+          (firstn
+             (Datatypes.length (pat_fv p) + Datatypes.length (bnd_t t1))
+             (skipn (Datatypes.length (bnd_t tm)) l)))))
+
+
+    match_val_single gamma_valid pd all_unif vt v
+    (has_type_valid gamma_valid
+       (alpha_t_aux tm (firstn (Datatypes.length (bnd_t tm)) l)) v t)
+    (term_rep vv tm v t0) p0
+
+
+
+      match_val_single gamma_valid pd all_unif vt v
+      (has_type_valid gamma_valid tm v t0) (term_rep vv tm v t0) p
+
+
+      match_val_single gamma_valid pd all_unif vt v
+    (has_type_valid gamma_valid
+       (alpha_t_aux tm (firstn (Datatypes.length (bnd_t tm)) l)) v t)
+    (term_rep vv (alpha_t_aux tm (firstn (Datatypes.length (bnd_t tm)) l)) v
+       t) p0
+
+
+
+    + rewrite H with(l:=(firstn (Datatypes.length (bnd_t tm)) l))
+      (Hty2:=t).
+      destruct (match_val_single gamma_valid pd all_unif vt v
+      (has_type_valid gamma_valid tm v t0)
+      (term_rep vv (alpha_t_aux tm (firstn (Datatypes.length (bnd_t tm)) l)) v
+         t) p) eqn : Hm.
+      
+      
+      (has_type_valid gamma_valid
+      (alpha_t_aux tm (firstn (Datatypes.length (bnd_t tm)) l)) v t)).
+
+
+    match_val_single gamma_valid pd all_unif vt v
+    (has_type_valid gamma_valid tm v t0) (term_rep vv tm v t0) p
+
+
+
+    match_val_single gamma_valid pd all_unif vt v
+     (has_type_valid gamma_valid
+        (alpha_t_aux tm (firstn (Datatypes.length (bnd_t tm)) l)) v t)
+     (term_rep vv (alpha_t_aux tm (firstn (Datatypes.length (bnd_t tm)) l)) v
+        t) p0
+    
+    
+    
+    reflexivity.
 
 
 
